$r_i^{(s)}$ $\in$ [0,1] and $\phi^{(t)}$= $\sum_{i}w_i^{(t)}$ be the potential function. \\
$\implies$ \\
$$\phi^{(t+1)}= \sum_{i}w_i^{(t+1)} $$\\
=$$\sum_{i} w_i^{(t)}(1+\alpha r_i^{(t)})$$ \\
Since,$ p_i^{(t)}$=$w_i^{(t)}$/$\phi_i^{(t)}$ \\
=$$\sum_{i}w_i^{(t)} + \alpha\cdot \sum_{i=1}^{n} p_i^{(t)}\cdot\phi^{(t)}\cdot r_i^{(t)} $$\\
=$$\phi^{(t)}+ \alpha\cdot\phi^{(t)}\sum_{s=1}^{t}p_i^{(t)}r_i^{(t)}$$
 =$$\phi_i^{(t)} (1 +\alpha\sum_{(i=1)}^{n}p_i^{(t)}r_i^{(t)}) \leq  \phi_i^{(t)} (1 +\alpha\sum_{(i=1)}^{n}\sum_{s=1}^{t}p_i^{(s)}r_i^{(s)})$$
Using, i+x$\leq e^x $
$$\leq \phi^{(t)}\cdot e^{\alpha\sum_{i}\sum_{s=1}^{t}p_i^{(s)}r_i^{(s)}}$$ \\

After T rounds, by simple induction for t, it can be shown that,
\begin{equation}
	\phi^{(T)}\leq \phi^{(1)}\cdot e^{\alpha\sum_{s=1}^{t}\sum_{i=1}^{n}p_i^{(s)}r_i^{(s)}}
\end{equation}
\\\\
Also, $\phi^{(1)}=n $ and for every i, 
$\phi^{(T)}\geq w_i^{(T)} = \prod_{s=1}^t(1+\alpha\cdot r_i^{(s)})$ ( By induction).
Since, $ 1+\alpha x \geq (1 +\alpha)^{x} $, we have:
\begin{equation}
	\phi^{(T)} \geq (1+\alpha)^{\sum_s{r_i^{(s)}}}
\end{equation}

Hence, we have the bound for the potential function from 1 and 2, \\
$$n\cdot e^{\alpha\sum_{i=1}^{n}\sum_{s=1}^{t}p_i^{t}r_i^{(s)}} \geq \phi^{(t)} \geq (1+\alpha)^{\sum_{s=1}^{t}r_i^{(s)}}$$
Taking logarithm, \\
$$ln(n) + \alpha\sum_{i=1}^{n}\sum_{s=1}^{t}p_i^{(s)}r_i^{(s)} \geq ln(1+\alpha)\cdot \sum_{s=1}^{t} r_i^{(s)}  $$
Also, $ ln(1+\alpha) \geq \alpha- \alpha^{2} $
Hence, \\

$$\sum_{i}\sum_{s=1}^{t}p_i^{s}r_i^{s} \geq -ln(n)/\alpha + \sum_{s=1}^{t}r_j^{s} (1-\alpha) $$